src/Crypto/Digests.dfy
@@ -1,16 +1,24 @@
 include "../StandardLibrary/StandardLibrary.dfy"
 
 module {:extern "Digests"} Digests {
-    import opened StandardLibrary
-    import opened UInt = StandardLibrary.UInt
+  import opened StandardLibrary
+  import opened UInt = StandardLibrary.UInt
 
-    datatype {:extern "HMAC_ALGORITHM"} HMAC_ALGORITHM = HmacSHA256 | HmacSHA384 | HmacNOSHA
+  datatype {:extern "KEY_DERIVATION_ALGORITHM"} KEY_DERIVATION_ALGORITHM = HKDF_WITH_SHA_384 | HKDF_WITH_SHA_256 | IDENTITY
 
-    // Hash length in octets (bytes), e.g. HashLength(SHA256) = 256 = 32 * 8
-    function {:axiom} HashLength(algorithm: HMAC_ALGORITHM): (n: nat)
-        ensures algorithm == HmacSHA256 ==> n == 32
-        ensures algorithm == HmacSHA384 ==> n == 48
+  // Hash length in octets (bytes), e.g. HashLength(SHA256) = 256 = 32 * 8
+  function HashLength(algorithm: KEY_DERIVATION_ALGORITHM): (n: nat)
+    ensures algorithm == HKDF_WITH_SHA_256 ==> n == 32
+    ensures algorithm == HKDF_WITH_SHA_384 ==> n == 48
+    ensures algorithm == IDENTITY ==> n == 0
+  {
+    match algorithm {
+      case HKDF_WITH_SHA_256 => 32
+      case HKDF_WITH_SHA_384 => 48
+      case IDENTITY => 0
+    }
+  }
 
-    function {:axiom} Hash(algorithm: HMAC_ALGORITHM, key: seq<uint8>, message: seq<uint8>): (s: seq<uint8>)
-        ensures |s| == HashLength(algorithm)
+    function {:axiom} Hash(algorithm: KEY_DERIVATION_ALGORITHM, key: seq<uint8>, message: seq<uint8>): (s: seq<uint8>)
+      ensures |s| == HashLength(algorithm)
 }
