test/hkdf/HKDF.dfy
@@ -22,7 +22,7 @@ module {:extern "TestHKDF"} TestHKDF {
                                    0x5a, 0x4c, 0x5d, 0xb0, 0x2d, 0x56, 0xec, 0xc4, 0xc5, 0xbf, 0x34,
                                    0x00, 0x72, 0x08, 0xd5, 0xb8, 0x87, 0x18, 0x58, 0x65 ];
 
-    var okm := hkdf(HmacSHA256, Some(tv_salt), tv_ikm, tv_info, 42);
+    var okm := hkdf(HKDF_WITH_SHA_256, Some(tv_salt), tv_ikm, tv_info, 42);
     return RequireEqual(tv_okm_desired[..], okm[..]);
   }
 
@@ -57,7 +57,7 @@ module {:extern "TestHKDF"} TestHKDF {
                                  0x42, 0xa3, 0x82, 0x2e, 0xd7, 0xa6, 0xdf, 0xf1, 0x6c, 0x3b, 0x61, 0x3b,
                                  0x58, 0x9e, 0xcf, 0x0f, 0x71, 0x0b, 0xdf, 0x2b, 0x15, 0x39 ];
 
-    var okm := hkdf(HmacSHA256, Some(tv_salt), tv_ikm, tv_info, 82);
+    var okm := hkdf(HKDF_WITH_SHA_256, Some(tv_salt), tv_ikm, tv_info, 82);
     return RequireEqual(tv_okm_desired[..], okm[..]);
   }
 
@@ -75,7 +75,7 @@ module {:extern "TestHKDF"} TestHKDF {
                                  0x87, 0x9e, 0xc3, 0x45, 0x4e, 0x5f, 0x3c, 0x73, 0x8d, 0x2d, 0x9d,
                                  0x20, 0x13, 0x95, 0xfa, 0xa4, 0xb6, 0x1a, 0x96, 0xc8 ];
 
-    var okm := hkdf(HmacSHA256, tv_salt, tv_ikm, tv_info, 42);
+    var okm := hkdf(HKDF_WITH_SHA_256, tv_salt, tv_ikm, tv_info, 42);
     return RequireEqual(tv_okm_desired[..], okm[..]);
   }
 
@@ -93,7 +93,7 @@ module {:extern "TestHKDF"} TestHKDF {
                                  0xbf, 0x36, 0x9f, 0x39, 0x4c, 0xfa, 0xb4, 0x36, 0x85, 0xf7, 0x48,
                                  0xb6, 0x45, 0x77, 0x63, 0xe4, 0xf0, 0x20, 0x4f, 0xc5 ];
 
-    var okm := hkdf(HmacSHA384, Some(tv_salt), tv_ikm, tv_info, 42);
+    var okm := hkdf(HKDF_WITH_SHA_384, Some(tv_salt), tv_ikm, tv_info, 42);
     return RequireEqual(tv_okm_desired[..], okm[..]);
   }
 
@@ -128,7 +128,7 @@ module {:extern "TestHKDF"} TestHKDF {
                                  0x99, 0x4f, 0xdb, 0xd6, 0xf4, 0xc0, 0x9c, 0x55, 0x00, 0xdc, 0xa2, 0x4a,
                                  0x56, 0x22, 0x2f, 0xea, 0x53, 0xd8, 0x96, 0x7a, 0x8b, 0x2e ];
 
-    var okm := hkdf(HmacSHA384, Some(tv_salt), tv_ikm, tv_info, 82);
+    var okm := hkdf(HKDF_WITH_SHA_384, Some(tv_salt), tv_ikm, tv_info, 82);
     return RequireEqual(tv_okm_desired[..], okm[..]);
   }
 
@@ -146,7 +146,7 @@ module {:extern "TestHKDF"} TestHKDF {
                                  0xa7, 0xab, 0xc7, 0x43, 0xfa, 0xde, 0x9b, 0x24, 0x2d, 0xaa, 0xcc,
                                  0x1c, 0xea, 0x56, 0x70, 0x41, 0x5b, 0x52, 0x84, 0x9c ];
 
-    var okm := hkdf(HmacSHA384, tv_salt, tv_ikm, tv_info, 42);
+    var okm := hkdf(HKDF_WITH_SHA_384, tv_salt, tv_ikm, tv_info, 42);
     return RequireEqual(tv_okm_desired[..], okm[..]);
   }
 
@@ -589,7 +589,7 @@ module {:extern "TestHKDF"} TestHKDF {
       0xf3, 0x05, 0xfc, 0xac, 0x34, 0x2b, 0xf0, 0x95, 0x47, 0x31, 0x63, 0xe9, 0x9f, 0x4b, 0x9d, 0xc2, 0x44, 0xd4, 0xc3,
       0xbb, 0x65, 0xc3, 0x9f, 0xcf, 0x3e, 0xe3, 0x99, 0x89, 0x33, 0x61, 0x46, 0xdc, 0xb7, 0xba, 0x76 ];
 
-    var okm := hkdf(HmacSHA256, Some(tv_salt), tv_ikm, tv_info, 8129);
+    var okm := hkdf(HKDF_WITH_SHA_256, Some(tv_salt), tv_ikm, tv_info, 8129);
     return RequireEqual(tv_okm_desired[..], okm[..]);
   }
 }
